add a peek operation

src/3d/prelude/extern/EverParse3d.InputStream.Extern.fst
@@ -216,6 +216,38 @@ let read
   );
   res
 
+inline_for_extraction
+noextract
+let peep
+    (#[FStar.Tactics.Typeclasses.tcresolve ()] _extra_t: Aux.extra_t)
+    (x: t)
+    (position: LPE.pos_t)
+    (n: U64.t)
+:   HST.Stack (B.buffer U8.t)
+    (requires (fun h ->
+      live x h /\
+      U64.v position == Seq.length (get_read x h)
+    ))
+    (ensures (fun h dst' h' ->
+      let s = get_remaining x h in
+      B.modifies B.loc_none h h' /\
+      ((~ (B.g_is_null dst')) ==> (
+        Seq.length (get_remaining x h) >= U64.v n /\
+        B.as_seq h' dst' `Seq.equal` Seq.slice s 0 (U64.v n) /\
+        B.live h' dst' /\
+        footprint x `B.loc_includes` B.loc_buffer dst'
+      ))
+    ))
+=
+  let h0 = HST.get () in
+  if has x () position n
+  then begin
+    let h1 = HST.get () in
+    preserved x B.loc_none h0 h1;
+    Aux.peep x.Aux.base n
+  end else
+    B.null
+
 #pop-options
 
 inline_for_extraction
