src/3d/prelude/extern/EverParse3d.Actions.All.fst
@@ -2,7 +2,7 @@ module EverParse3d.Actions.All
 
 let _ = EverParse3d.Actions.BackendFlagValue.backend_flag_value
 
-let ___PUINT8 = unit
+let ___PUINT8 = LowStar.Buffer.buffer FStar.UInt8.t
 
 let action_field_ptr u = false_elim ()
 
