src/3d/prelude/extern/EverParse3d.InputStream.Extern.Base.fsti
@@ -94,6 +94,25 @@ val read:
       get_remaining x h' `Seq.equal` Seq.slice s (U64.v n) (Seq.length s)
     ))
 
+val peep:
+    (#[FStar.Tactics.Typeclasses.tcresolve ()] _extra_t: extra_t) ->
+    (x: t) ->
+    (n: U64.t) ->
+    HST.Stack (B.buffer U8.t)
+    (requires (fun h ->
+      live x h /\
+      Seq.length (get_remaining x h) >= U64.v n
+    ))
+    (ensures (fun h dst' h' ->
+      let s = get_remaining x h in
+      B.modifies B.loc_none h h' /\
+      ((~ (B.g_is_null dst')) ==> (
+        B.as_seq h' dst' `Seq.equal` Seq.slice s 0 (U64.v n) /\
+        B.live h' dst' /\
+        footprint x `B.loc_includes` B.loc_buffer dst'
+      ))
+    ))
+
 val skip:
     (#[FStar.Tactics.Typeclasses.tcresolve ()] _extra_t: extra_t) ->
     (x: t) ->
